Update confluence to be up-to renamings in contexts

pcuic/theories/PCUICConfluence.v
@@ -802,6 +802,7 @@ Section RedConfluence.
   Section OnOne_local_2.
     Context (P : forall (Γ : context), option (term * term) -> term -> term -> Type).
 
+    (** We allow alpha-conversion *)
     Inductive OnOne2_local_env : context -> context -> Type :=
     | localenv2_cons_abs Γ na t t' :
         P Γ None t t' ->
@@ -814,6 +815,46 @@ Section RedConfluence.
         OnOne2_local_env (Γ ,, d) (Γ' ,, d).
   End OnOne_local_2.
 
+  Inductive clos_refl_trans_ctx_decl (R : relation context_decl) (x : context_decl) : context_decl → Type :=
+    rt_ctx_decl_step : ∀ y, R x y → clos_refl_trans_ctx_decl R x y
+  | rt_ctx_decl_refl y : decl_body x = decl_body y -> decl_type x = decl_type y -> clos_refl_trans_ctx_decl R x y
+  | rt_ctx_decl_trans : ∀ y z, clos_refl_trans_ctx_decl R x y → clos_refl_trans_ctx_decl R y z → clos_refl_trans_ctx_decl R x z.
+
+  Inductive eq_context_upto_names : context -> context -> Type :=
+  | eq_context_nil : eq_context_upto_names [] []
+  | eq_context_decl x y Γ Γ' :
+      decl_body x = decl_body y -> decl_type x = decl_type y ->
+      eq_context_upto_names Γ Γ' ->
+      eq_context_upto_names (Γ ,, x) (Γ' ,, y).
+
+  Global Instance eq_context_upto_names_refl : Reflexive eq_context_upto_names.
+  Proof. intros Γ; induction Γ; constructor; auto. Qed.
+
+  Global Instance eq_context_upto_names_sym : Symmetric eq_context_upto_names.
+  Proof. intros Γ Γ' H; induction H; constructor; auto. Qed.
+
+  Global Instance eq_context_upto_names_trans : Transitive eq_context_upto_names.
+  Proof.
+    intros Γ0 Γ1 Γ2 H.
+    induction H in Γ2 |- *; intros H2; depelim H2; econstructor; auto.
+    etransitivity; eauto.
+    etransitivity; eauto.
+  Qed.
+
+  Inductive clos_refl_trans_ctx (R : relation context) (x : context) : context → Type :=
+  | rt_ctx_step : ∀ y, R x y → clos_refl_trans_ctx R x y
+  | rt_ctx_refl y : eq_context_upto_names x y -> clos_refl_trans_ctx R x y
+  | rt_ctx_trans : ∀ y z, clos_refl_trans_ctx R x y → clos_refl_trans_ctx R y z → clos_refl_trans_ctx R x z.
+
+  Global Instance clos_refl_trans_ctx_refl R :
+    Reflexive (clos_refl_trans_ctx R).
+  Proof. intros HR. constructor 2. reflexivity. Qed.
+
+  Global Instance clos_refl_trans_ctx_trans R : Transitive (clos_refl_trans_ctx R).
+  Proof.
+    intros x y z; econstructor 3; eauto.
+  Qed.
+
   Definition red1_ctx := (OnOne2_local_env (on_one_decl (fun Δ t t' => red1 Σ Δ t t'))).
 
   Definition red1_rel : relation (context * term) :=
@@ -822,7 +863,6 @@ Section RedConfluence.
 
   Definition red_ctx : relation context :=
     All2_local_env (on_decl (fun Γ Δ t u => red Σ Γ t u)).
-
 
   Lemma red1_ctx_pred1_ctx Γ Γ' : red1_ctx Γ Γ' -> pred1_ctx Σ Γ Γ'.
   Proof.
@@ -847,11 +887,11 @@ Section RedConfluence.
     now apply pred1_red in redt.
   Qed.
 
-  Definition red_rel' :=
+  Definition red_rel_ctx :=
     fun '(Γ, t) '(Δ, u) =>
       (red Σ Γ t u * red_ctx Γ Δ)%type.
 
-  Lemma pred1_red' Γ Γ' : forall M N, pred1 Σ Γ Γ' M N -> red_rel' (Γ, M) (Γ', N).
+  Lemma pred1_red' Γ Γ' : forall M N, pred1 Σ Γ Γ' M N -> red_rel_ctx (Γ, M) (Γ', N).
   Proof.
     intros * Hred.
     split. apply (pred1_red wfΣ _ _ _ _ Hred). (* apply (pred1_red_r wfΣ _ _ _ _ Hred). *)
@@ -910,18 +950,26 @@ Section RedConfluence.
     - red in p.
       induction p. repeat constructor. firstorder.
       constructor 2.
-      etransitivity; eauto.
+      econstructor 3 with (Γ ,, vass na y); auto.
     - subst.
       induction a. repeat constructor. firstorder.
       constructor 2.
-      etransitivity; eauto.
+      econstructor 3 with (Γ ,, vdef na y t'); auto.
     - subst.
       induction a. constructor. constructor. red. right. firstorder.
       constructor 2.
-      etransitivity; eauto.
+      econstructor 3 with (Γ ,, vdef na b' y); auto.
     - clear H. induction IHOnOne2_local_env. constructor. now constructor 3.
       constructor 2.
-      etransitivity; eauto.
+      eapply transitivity. eauto. auto.
+  Qed.
+
+  Lemma clos_rt_OnOne2_local_env_ctx_incl R :
+    inclusion (clos_refl_trans (OnOne2_local_env (on_one_decl R)))
+              (clos_refl_trans_ctx (OnOne2_local_env (on_one_decl R))).
+  Proof.
+    intros x y H.
+    induction H; firstorder; try solve[econstructor; eauto].
   Qed.
 
   Lemma OnOne2_local_env_impl R S :
@@ -933,79 +981,158 @@ Section RedConfluence.
     induction H'; try solve [econstructor; firstorder].
   Qed.
 
-  Lemma red_ctx_clos_rt_red1_ctx : inclusion red_ctx (clos_refl_trans red1_ctx).
+  Lemma red_ctx_clos_rt_red1_ctx : inclusion red_ctx (clos_refl_trans_ctx red1_ctx).
   Proof.
     intros x y H.
     induction H; try firstorder.
     red in p.
     transitivity (Γ ,, vass na t').
-    eapply clos_rt_OnOne2_local_env_incl. constructor. red.
+    eapply clos_rt_OnOne2_local_env_ctx_incl, clos_rt_OnOne2_local_env_incl. constructor. red.
     eapply red_alt in p; eauto.
     clear p H.
-    induction IHAll2_local_env. constructor. constructor 3. apply r.
-    constructor 2.
+    transitivity (Γ ,, vass na' t').
+    { constructor 2. repeat constructor; auto. apply reflexivity. }
+    induction IHAll2_local_env; try solve[repeat constructor; auto].
     etransitivity; eauto.
-
     apply red_alt in a. apply red_alt in b0.
     transitivity (Γ ,, vdef na b t').
-    - eapply clos_rt_OnOne2_local_env_incl. constructor 2. red.
+    - eapply clos_rt_OnOne2_local_env_ctx_incl, clos_rt_OnOne2_local_env_incl. constructor 2. red.
       right. split; auto.
     - transitivity (Γ ,, vdef na b' t').
-      eapply clos_rt_OnOne2_local_env_incl.
+      eapply clos_rt_OnOne2_local_env_ctx_incl, clos_rt_OnOne2_local_env_incl.
       constructor 2. red. left; split; auto.
       clear -IHAll2_local_env.
-      induction IHAll2_local_env.
-      * constructor. now constructor.
-      * constructor 2.
-      * etransitivity; eauto.
+      transitivity (Γ ,, vdef na' b' t').
+      { constructor 2. repeat constructor; auto. apply reflexivity. }
+      induction IHAll2_local_env; try solve[repeat constructor; auto].
+      etransitivity; eauto.
   Qed.
 
-  Lemma clos_rt_red1_rel_red_rel : inclusion red_rel' (clos_refl_trans red1_rel).
+  Inductive clos_refl_trans_ctx_t (R : relation (context * term)) (x : context * term) : context * term → Type :=
+  | rt_ctx_t_step : ∀ y, R x y → clos_refl_trans_ctx_t R x y
+  | rt_ctx_t_refl y : eq_context_upto_names (fst x) (fst y) -> snd x = snd y -> clos_refl_trans_ctx_t R x y
+  | rt_ctx_t_trans : ∀ y z, clos_refl_trans_ctx_t R x y → clos_refl_trans_ctx_t R y z → clos_refl_trans_ctx_t R x z.
+
+  Global Instance clos_refl_trans_ctx_t_refl R :
+    Reflexive (clos_refl_trans_ctx_t R).
+  Proof. intros HR. constructor 2. reflexivity. auto. Qed.
+
+  Global Instance clos_refl_trans_ctx_t_trans R : Transitive (clos_refl_trans_ctx_t R).
+  Proof.
+    intros x y z; econstructor 3; eauto.
+  Qed.
+
+  Definition clos_rt_ctx_t_monotone (R S : relation _) :
+    inclusion R S -> inclusion (clos_refl_trans_ctx_t R) (clos_refl_trans_ctx_t S).
+  Proof.
+    move => incls x y.
+    induction 1; solve [econstructor; eauto].
+  Qed.
+
+  Lemma clos_rt_ctx_t_disjunction_left (R S : relation _) :
+    inclusion (clos_refl_trans_ctx_t R)
+              (clos_refl_trans_ctx_t (relation_disjunction R S)).
+  Proof.
+    apply clos_rt_ctx_t_monotone.
+    intros x y H; left; exact H.
+  Qed.
+
+  Lemma clos_rt_ctx_t_disjunction_right (R S : relation _) :
+    inclusion (clos_refl_trans_ctx_t S)
+              (clos_refl_trans_ctx_t (relation_disjunction R S)).
+  Proof.
+    apply clos_rt_ctx_t_monotone.
+    intros x y H; right; exact H.
+  Qed.
+
+  Lemma clos_refl_trans_ctx_t_prod_l (R : relation _) (S : relation _) :
+    (forall x y b, R x y -> S (x, b) (y, b)) ->
+    forall x y b,
+      clos_refl_trans_ctx R x y ->
+      clos_refl_trans_ctx_t S (x, b) (y, b).
+  Proof.
+    intros. induction X0; try solve [econstructor; eauto].
+  Qed.
+
+  Lemma clos_refl_trans_ctx_t_prod_r (R : relation term) (S : relation (context * term)) a :
+    (forall x y, R x y -> S (a, x) (a, y)) ->
+    forall x y,
+      clos_refl_trans R x y ->
+      clos_refl_trans_ctx_t S (a, x) (a, y).
+  Proof.
+    intros. induction X0; try solve [econstructor; eauto].
+    constructor 2. simpl. apply reflexivity. reflexivity.
+  Qed.
+
+  Lemma clos_rt_red1_rel_ctx_rt_ctx_red1_rel : inclusion red_rel_ctx (clos_refl_trans_ctx_t red1_rel).
   Proof.
     move=> [Γ t] [Δ u] [redt redctx].
     eapply red_alt in redt.
     eapply clos_rt_rt1n_iff in redt.
     induction redt.
     induction redctx; try solve [constructor; eauto].
+    - constructor 2; simpl; apply reflexivity.
     - red in p.
       etransitivity.
-      * eapply clos_rt_disjunction_right.
-        eapply red_alt in p. instantiate (1:= (Γ',, vass na t', x)).
-        eapply clos_refl_trans_prod_l. intros. split; eauto.
+      * eapply clos_rt_ctx_t_disjunction_right.
+        eapply red_alt in p. instantiate (1:= (Γ',, vass na' t', x)).
+        eapply clos_refl_trans_ctx_t_prod_l. intros. split; eauto.
+        transitivity (Γ ,, vass na' t).
+        constructor 2. repeat constructor; apply reflexivity.
         apply red_ctx_clos_rt_red1_ctx. constructor; auto.
         red. apply red_alt; auto.
-      * clear p. eapply clos_rt_disjunction_right.
-        eapply clos_refl_trans_prod_l. intros. split; eauto.
-        constructor 2.
+      * clear p. eapply clos_rt_ctx_t_disjunction_right.
+        constructor 2; simpl; apply reflexivity.
     - red in p.
       destruct p.
       eapply red_alt in r. eapply red_alt in r0.
       etransitivity.
-      * eapply clos_rt_disjunction_right.
+      * eapply clos_rt_ctx_t_disjunction_right.
         instantiate (1:= (Γ',, vdef na b' t', x)).
-        eapply clos_refl_trans_prod_l. intros. split; eauto.
+        eapply clos_refl_trans_ctx_t_prod_l. intros. split; eauto.
         apply red_ctx_clos_rt_red1_ctx. constructor; auto.
         red. split; apply red_alt; auto.
       * clear r r0.
-        eapply clos_rt_disjunction_right.
-        eapply clos_refl_trans_prod_l. intros. split; eauto.
-        constructor 2.
+        eapply clos_rt_ctx_t_disjunction_right.
+        eapply clos_refl_trans_ctx_t_prod_l. intros. split; eauto.
+        constructor 2. constructor; auto. apply reflexivity.
     - transitivity (Γ, y).
-      * eapply clos_rt_disjunction_left.
-        eapply clos_refl_trans_prod_r. intros. split; eauto.
+      * eapply clos_rt_ctx_t_disjunction_left.
+        eapply clos_refl_trans_ctx_t_prod_r. intros. split; eauto.
         constructor. apply r.
       * apply IHredt.
   Qed.
 
-  Lemma pred_rel_confluent : confluent red1_rel.
+  Definition red1_rel_alpha : relation (context * term) :=
+    relation_disjunction (fun '(Γ, t) '(Δ, u) => (red1 Σ Γ t u * (Γ = Δ)))%type
+     (relation_disjunction
+        (fun '(Γ, t) '(Δ, u) => ((red1_ctx Γ Δ * (t = u))))
+        (fun '(Γ, t) '(Δ, u) => ((eq_context_upto_names Γ Δ * (t = u)))))%type.
+
+  Lemma clos_rt_red1_rel_rt_ctx : inclusion (clos_refl_trans red1_rel) (clos_refl_trans_ctx_t red1_rel).
+  Proof.
+    intros x y H.
+    induction H.
+    - destruct x, y. constructor. auto.
+    - constructor 2; apply reflexivity.
+    - econstructor 3; eauto.
+  Qed.
+
+  Lemma pred_rel_confluent : confluent red1_rel_alpha.
   Proof.
     notypeclasses refine (fst (sandwich _ _ _ _) _).
     3:eapply pred1_rel_confluent; eauto.
     intros [ctx t] [ctx' t'].
-    rewrite /red1_rel /pred1_rel /=.
-    intros [[l <-]|[r <-]].
+    rewrite /red1_rel_alpha /pred1_rel /=.
+    intros [[l <-]|[[r <-]|[r <-]]].
     - now eapply red1_pred1.
     - eapply pred1_refl_gen. now apply red1_ctx_pred1_ctx.
+    - eapply pred1_refl_gen.
+      induction r.
+      * constructor.
+      * destruct x as [na [b|] ty], y as [na' [b'|] ty']; simpl in *; noconf e; try noconf e0.
+        constructor; auto. red. split; now apply pred1_refl_gen.
+        constructor; auto. red; now apply pred1_refl_gen.
     - intros x y pred. red in pred.
       eapply pred1_red' in pred; auto.
       destruct pred.
@@ -1015,8 +1142,13 @@ Section RedConfluence.
       eapply clos_refl_trans_prod_r. intros. split; eauto.
       now eapply red_alt in r.
       eapply clos_rt_disjunction_right.
-      eapply clos_refl_trans_prod_l. intros. split; eauto.
-      now eapply red_ctx_clos_rt_red1_ctx.
+      eapply (clos_refl_trans_prod_l (fun x y => red1_ctx x y + eq_context_upto_names x y))%type.
+      intros. red. destruct X; intuition auto.
+      clear r.
+      apply red_ctx_clos_rt_red1_ctx in r0.
+      induction r0. constructor; auto.
+      constructor. auto.
+      now transitivity y.
   Qed.
 
   Lemma clos_refl_trans_out Γ x y :
@@ -1091,7 +1223,6 @@ Section RedConfluence.
     - eapply red_trans; eauto.
   Qed.
 
-
   Lemma clos_red_rel_out x y :
     clos_refl_trans red1_rel x y ->
     clos_refl_trans pred1_rel x y.
@@ -1105,17 +1236,67 @@ Section RedConfluence.
     eapply pred1_refl_gen. now eapply red1_ctx_pred1_ctx.
   Qed.
 
+  Lemma red1_rel_alpha_red1_rel : inclusion (clos_refl_trans red1_rel_alpha) (clos_refl_trans_ctx_t red1_rel).
+  Proof.
+    intros x y H.
+    induction H.
+    - destruct x, y.
+      destruct r. destruct p; subst.
+      constructor. firstorder.
+      destruct r. destruct p; subst.
+      constructor. firstorder.
+      destruct p; subst.
+      constructor 2. simpl. auto. reflexivity.
+    - constructor 2; reflexivity.
+    - econstructor 3; eauto.
+  Qed.
+
+  Lemma red1_rel_alpha_red1_rel_inv : inclusion (clos_refl_trans_ctx_t red1_rel) (clos_refl_trans red1_rel_alpha).
+  Proof.
+    intros x y H.
+    induction H.
+    - destruct x, y.
+      destruct r. destruct p; subst.
+      constructor. firstorder.
+      destruct p. subst.
+      constructor. firstorder.
+    - destruct x, y. simpl in *.
+      subst. constructor. firstorder.
+    - econstructor 3; eauto.
+  Qed.
+
+  Definition eqb_context_decl (x y : context_decl) :=
+    let (na, b, ty) := x in
+    let (na', b', ty') := y in
+    eqb na na' && eqb b b' && eqb ty ty'.
+
+  Instance eq_ctx : ReflectEq context_decl.
+  Proof.
+    refine {| eqb := eqb_context_decl |}.
+    intros.
+    destruct x as [na b ty], y as [na' b' ty']. cbn -[eqb].
+    destruct (eqb_spec na na'); subst;
+    destruct (eqb_spec b b'); subst;
+    destruct (eqb_spec ty ty'); subst; constructor; congruence.
+  Qed.
+
+  Instance eqb_ctx : ReflectEq context := _.
+
   Lemma clos_red_rel_out_inv x y :
     clos_refl_trans pred1_rel x y ->
-    clos_refl_trans red1_rel x y.
+    clos_refl_trans red1_rel_alpha x y.
   Proof.
     induction 1.
     red in r.
     destruct x as [Γ t], y as [Δ u]; simpl in *.
-    pose proof (pred1_red wfΣ _ _ _ _ r).
-    apply clos_rt_red1_rel_red_rel. red. split; auto.
-    eapply pred1_pred1_ctx in r.
-    now apply pred1_ctx_red_ctx.
+    pose proof (pred1_pred1_ctx _ r).
+    apply red1_rel_alpha_red1_rel_inv.
+    transitivity (Γ, u).
+    eapply clos_refl_trans_ctx_t_prod_r. intros. red. left. split; eauto.
+    apply red_alt. now apply pred1_red in r.
+    eapply clos_refl_trans_ctx_t_prod_l. intros. red. right. split; eauto.
+    now apply red_ctx_clos_rt_red1_ctx, pred1_ctx_red_ctx.
+
     constructor 2.
     etransitivity; eauto.
   Qed.
@@ -1143,7 +1324,7 @@ Section RedConfluence.
     eapply red_red_ctx; eauto.
   Qed.
 
-  Lemma clos_red_rel_out' x y :
+  Lemma clos_rt_red1_rel_red1 x y :
     clos_refl_trans red1_rel x y ->
     red_ctx (fst x) (fst y) *
     clos_refl_trans (red1 Σ (fst x)) (snd x) (snd y).
@@ -1166,6 +1347,137 @@ Section RedConfluence.
         eapply red_red_ctx; eauto.
         apply red1_ctx_pred1_ctx in r.
         now apply pred1_ctx_red_ctx in r.
+  Qed.
+
+  Lemma decl_body_eq_context_upto_names Γ Γ' n d :
+    option_map decl_body (nth_error Γ n) = Some d ->
+    eq_context_upto_names Γ Γ' ->
+    option_map decl_body (nth_error Γ' n) = Some d.
+  Proof.
+    move: Γ' n d; induction Γ; destruct n; simpl; intros; try congruence.
+    noconf H. depelim H0. simpl. now rewrite -e.
+    depelim H0. simpl. apply IHΓ; auto.
+  Qed.
+
+  Lemma decl_type_eq_context_upto_names Γ Γ' n d :
+    option_map decl_type (nth_error Γ n) = Some d ->
+    eq_context_upto_names Γ Γ' ->
+    option_map decl_type (nth_error Γ' n) = Some d.
+  Proof.
+    move: Γ' n d; induction Γ; destruct n; simpl; intros; try congruence.
+    noconf H. depelim H0. simpl. now rewrite -e0.
+    depelim H0. simpl. apply IHΓ; auto.
+  Qed.
+
+  Lemma eq_context_upto_names_app Γ Γ' Δ :
+    eq_context_upto_names Γ Γ' ->
+    eq_context_upto_names (Γ ,,, Δ) (Γ' ,,, Δ).
+  Proof.
+    induction Δ; auto. constructor; auto.
+  Qed.
+
+  Lemma red1_eq_context_upto_names Γ Γ' t u :
+    eq_context_upto_names Γ Γ' ->
+    red1 Σ Γ t u ->
+    red1 Σ Γ' t u.
+  Proof.
+    move=> Hctx H.
+    revert Γ' Hctx.
+    induction H using red1_ind_all; intros Δ Hctx; try solve [repeat (econstructor; eauto)].
+    - constructor.
+      now eapply decl_body_eq_context_upto_names.
+    - constructor. apply (IHred1 (Δ ,, vass na N)). constructor; auto.
+    - constructor. apply (IHred1 (Δ ,, vdef na b t)). constructor; auto.
+    - constructor. solve_all.
+    - constructor. apply (IHred1 (Δ ,, vass na M1)). constructor; auto.
+    - constructor. solve_all.
+    - constructor. solve_all.
+    - eapply fix_red_body; solve_all.
+      eapply (b0 (Δ ,,, fix_context mfix0)).
+      now apply eq_context_upto_names_app.
+    - eapply cofix_red_ty; solve_all.
+    - eapply cofix_red_body; solve_all.
+      eapply (b0 (Δ ,,, fix_context mfix0)).
+      now apply eq_context_upto_names_app.
+  Qed.
+
+  Lemma clos_rt_red1_eq_context_upto_names Γ Γ' t u :
+    eq_context_upto_names Γ Γ' ->
+    clos_refl_trans (red1 Σ Γ) t u ->
+    clos_refl_trans (red1 Σ Γ') t u.
+  Proof.
+    intros HΓ H. move: H. apply clos_rt_monotone => x y.
+    now apply red1_eq_context_upto_names.
+  Qed.
+
+  Lemma red_eq_context_upto_names Γ Γ' t u :
+    eq_context_upto_names Γ Γ' ->
+    red Σ Γ t u ->
+    red Σ Γ' t u.
+  Proof.
+    intros HΓ H. apply red_alt in H. apply red_alt.
+    move: H. apply clos_rt_monotone => x y.
+    now apply red1_eq_context_upto_names.
+  Qed.
+
+  Lemma eq_context_upto_names_red_ctx Γ Δ Γ' Δ' :
+    eq_context_upto_names Γ Γ' ->
+    eq_context_upto_names Δ Δ' ->
+    red_ctx Γ Δ ->
+    red_ctx Γ' Δ'.
+  Proof.
+    intros.
+    induction H in H0, Δ, Δ', X |- *. depelim X. depelim H0. constructor.
+    destruct x as [na b ty], y as [na' b' ty']; simpl in *.
+    subst.
+    depelim X. depelim H0. hnf in H1. noconf H1.
+    red in o. simpl in *. subst.
+    destruct y as [? [b'|] ?]; noconf e.
+    constructor; auto. eapply IHeq_context_upto_names; eauto.
+    red. eapply red_eq_context_upto_names; eauto.
+    hnf in H1. noconf H1. destruct o. depelim H0. simpl in *.
+    destruct y as [? [b'|] ?]; noconf e. subst; simpl in *.
+    constructor. eapply IHeq_context_upto_names; eauto.
+    red.
+    split; eauto using red_eq_context_upto_names.
+  Qed.
+
+  Instance proper_red_ctx :
+    Proper (eq_context_upto_names ==> eq_context_upto_names ==> isEquiv) red_ctx.
+  Proof.
+    reduce_goal.
+    split.
+    intros. eapply eq_context_upto_names_red_ctx; eauto.
+    intros. symmetry in H, H0. eapply eq_context_upto_names_red_ctx; eauto.
+  Qed.
+
+  Lemma clos_rt_red1_alpha_out x y :
+    clos_refl_trans red1_rel_alpha x y ->
+    red_ctx (fst x) (fst y) *
+    clos_refl_trans (red1 Σ (fst x)) (snd x) (snd y).
+  Proof.
+    intros H.
+    eapply clos_rt_rt1n_iff in H.
+    induction H.
+    - split. red. induction (fst x) as [|[na [b|] ty] tl]; try constructor; hnf; eauto.
+      constructor 2.
+    - destruct x as [Γ t], y as [Δ u], z as [Δ' u']; simpl in *.
+      destruct IHclos_refl_trans_1n.
+      red in r. destruct r.
+      * destruct p. subst. split. auto.
+        transitivity u; auto. constructor. auto.
+      * destruct r. destruct p. subst. split.
+        apply red1_ctx_pred1_ctx in r.
+        apply pred1_ctx_red_ctx in r.
+        etransitivity; eauto.
+        apply red_alt in c. apply red_alt.
+        eapply red_red_ctx; eauto.
+        apply red1_ctx_pred1_ctx in r.
+        now apply pred1_ctx_red_ctx in r.
+        destruct p. subst.
+        split; auto.
+        eapply eq_context_upto_names_red_ctx. 3:eauto. now symmetry in e. reflexivity.
+        eapply clos_rt_red1_eq_context_upto_names; eauto. now symmetry in e.
   Qed.
 
   (* Lemma clos_red_rel_out_r x y : *)
@@ -1193,17 +1505,25 @@ Section RedConfluence.
   (*       now apply pred1_ctx_red_ctx in r. *)
   (* Qed. *)
 
+  Lemma clos_rt_red1_red1_rel_alpha Γ x y :
+    clos_refl_trans (red1 Σ Γ) x y -> clos_refl_trans red1_rel_alpha (Γ, x) (Γ, y).
+  Proof.
+    induction 1. constructor. red. left. firstorder.
+    constructor 2.
+    econstructor 3; eauto.
+  Qed.
+
   Lemma red1_confluent Γ : confluent (red1 Σ Γ).
   Proof.
     intros x y z.
     intros.
     pose proof (pred_rel_confluent (Γ, x) (Γ, y) (Γ, z)).
-    forward X1 by now eapply clos_refl_trans_out.
-    forward X1 by now eapply clos_refl_trans_out.
+    forward X1 by now eapply clos_rt_red1_red1_rel_alpha.
+    forward X1 by now eapply clos_rt_red1_red1_rel_alpha.
     destruct X1 as [[Δ nf] [redl redr]].
     exists nf.
-    eapply clos_red_rel_out' in redl.
-    eapply clos_red_rel_out' in redr. simpl in *.
+    eapply clos_rt_red1_alpha_out in redl.
+    eapply clos_rt_red1_alpha_out in redr. simpl in *.
     intuition auto.
   Qed.
 
@@ -1212,8 +1532,10 @@ Section RedConfluence.
     clos_refl_trans (red1 Σ Γ) t u.
   Proof.
     intros pred.
-    eapply (clos_red_rel_out' (Γ, t) (Γ, u)).
-    eapply clos_red_rel_out_inv.
+    eapply (clos_rt_red1_rel_red1 (Γ, t) (Γ, u)).
+    apply clos_refl_trans_out.
+    apply (clos_rt_red1_alpha_out (Γ, t) (Γ, u)).
+    apply clos_red_rel_out_inv.
     induction pred. constructor; auto. constructor 2.
     now transitivity (Γ, y).
   Qed.
